Add working model lemma

src/Std/Data/DHashMap/Internal/Defs.lean
@@ -481,7 +481,7 @@ def inter [BEq α] [Hashable α] (m₁ m₂ : Raw₀ α β) : Raw₀ α β :=
   if m₁.1.size ≤ m₂.1.size then m₁.filter fun k _ => m₂.contains k else interSmaller m₁ m₂
 
 /-- Internal implementation detail of the hash map -/
-def checkBEq [BEq α] [LawfulBEq α] [Hashable α] [∀ k, BEq (β k)] (m₁ m₂ : Raw₀ α β) : Bool :=
+def beq [BEq α] [LawfulBEq α] [Hashable α] [∀ k, BEq (β k)] (m₁ m₂ : Raw₀ α β) : Bool :=
   if m₁.1.size ≠ m₂.1.size then false else m₁.1.all (fun k v => m₂.get? k == some v)
 
 section
