src/Std/Data/DHashMap/Internal/WF.lean
@@ -275,6 +275,19 @@ theorem forIn_eq_forIn_toListModel {δ : Type w} {l : Raw α β} {m : Type w →
       · simp
       · simpa using ih'
 
+theorem all_toList {p : (a : α) → β a → Bool} {m : Raw α β}:
+    m.toList.all (fun x => p x.1 x.2) = m.all p := by
+  simp only [Raw.all, ForIn.forIn, Bool.not_eq_true, bind_pure_comp, map_pure, Id.run_bind]
+  rw [forIn_eq_forIn_toListModel, ← toList_eq_toListModel, forIn_eq_forIn']
+  induction m.toList with
+  | nil => simp only [all_nil, forIn'_nil, Id.run_pure]
+  | cons hd tl ih =>
+    simp only [forIn'_eq_forIn, List.all_cons]
+    by_cases h : p hd.fst hd.snd = false
+    · simp [h]
+    · simp only [forIn'_eq_forIn] at ih
+      simp [h, ih]
+
 end Raw
 
 namespace Raw₀
@@ -1486,5 +1499,24 @@ theorem Const.wf_insertManyIfNewUnit₀ [BEq α] [Hashable α] [EquivBEq α] [La
     {ρ : Type w} [ForIn Id ρ α] {m : Raw α (fun _ => Unit)} {h : 0 < m.buckets.size}
     {l : ρ} (h' : m.WF) : (Const.insertManyIfNewUnit ⟨m, h⟩ l).1.1.WF :=
   (Raw₀.Const.insertManyIfNewUnit ⟨m, h⟩ l).2 _ Raw.WF.insertIfNew₀ h'
+
+theorem toListModel_beq [BEq α] [LawfulBEq α] [Hashable α] [∀ k, BEq (β k)] {m₁ m₂ : Raw₀ α β}  (h₁ : Raw.WFImp m₁.1) (h₂ : Raw.WFImp m₂.1) :
+    beq m₁ m₂ = beqModel m₁.1.toList m₂.1.toList := by
+  rw [beq, beqModel]
+  split
+  case isTrue h =>
+    rw [Raw.size_eq_length, Raw.size_eq_length] at h
+    rw [Raw.toList_eq_toListModel, Raw.toList_eq_toListModel]
+    · simp only [ne_eq, h, not_false_eq_true, ↓reduceIte]
+    · exact h₂
+    · exact h₁
+  case isFalse h =>
+    rw [Raw.size_eq_length, Raw.size_eq_length] at h
+    simp [Raw.toList_eq_toListModel, h, ← Raw.all_toList]
+    congr
+    · ext x
+      rw [get?_eq_getValueCast? h₂]
+    · exact h₂
+    · exact h₁
 
 end Raw₀
